x86/Symbtablegenproof1.v
@@ -1196,4 +1196,3 @@ Proof.
       apply H1. apply in_map. auto.
 Qed.
       
-
